timing/examples/data_structures/linked_list/find_in_list.v
@@ -1,84 +1,391 @@
 Require Import linked_list.
-Require Import riscvTiming.
+Require Import RISCVTiming.
 Import RISCVNotations.
-Require Import timing_auto. 
+Require Import TimingAutomation.
+Require Import Arith.
+Require Import Lia ZifyN ZifyBool.
+Require Import Picinae_memsolve.
+Require Import Coq.Program.Equality.
 
-Module find_in_linked_listTime <: TimingModule.
-    Definition time_of_addr (s : store) (a : addr) : N :=
-        match neorv32_cycles_upper_bound s (linked_list_bin a) with
-        | Some x => x | _ => 999 end.
+Require Import Coq.Classes.RelationClasses.
 
+Ltac _noverlap_prepare :=
+  noverlap_prepare_unfold_hook; intros;
+   repeat
+   repeat
+    match goal with
+    | |- context [ ?M [Ⓓ?X + ?B + ?N := ?V ] ] =>
+          assert (TEMP:2^32-X < X) by lia; clear TEMP;
+          rewrite <- (Theory_RISCV.setmem_mod_l _ _ _ M (X + B + N) V);
+          replace (M [ⒹX + B ⊕ N := V ]) with
+          (M [ⒹB ⊖ (2 ^ 32 - X) ⊕ N := V ]) in * by (unfold msub; now psimpl);
+          simpl (2 ^ 32 - X)
+    | |- context [ ?M [Ⓓ?X + ?Y := ?V ] ] =>
+          assert (TEMP:2^32-X < X) by lia; clear TEMP;
+          rewrite <- Theory_RISCV.setmem_mod_l with (a := (X + Y)); replace
+          (X ⊕ Y) with (Y ⊖ (2 ^ 32 - X)) in * by now rewrite N.add_comm;
+          simpl (2 ^ 32 - X)
+    | |- context [ ?M Ⓓ[ ?X + ?B + ?N ] ] =>
+          assert (TEMP:2^32-X < X) by lia; clear TEMP;
+          rewrite <- (Theory_RISCV.getmem_mod_l _ _ _ M (X + B + N)); replace
+          (M Ⓓ[ X + B ⊕ N ]) with (M Ⓓ[ B ⊖ (2 ^ 32 - X) ⊕ N ]) in *
+          by (unfold msub; now psimpl);
+          simpl (2 ^ 32 - X)
+    | |- context [ ?M Ⓓ[ ?X + ?Y ] ] =>
+          assert (TEMP:2^32-X < X) by lia; clear TEMP;
+          rewrite <- Theory_RISCV.getmem_mod_l with (a := (X + Y)) in *; replace
+          (X ⊕ Y) with (Y ⊖ (2 ^ 32 - X)) in * by now rewrite N.add_comm;
+          simpl (2 ^ 32 - X)
+    end;
+    repeat match goal with [H:context[2^32-_]|-_] => simpl (2^32-_) in H end;
+   repeat
+    match goal with
+    | |- context [ ?N ⊖ 4294967248 ] =>
+          replace (N ⊖ 4294967248) with (48 ⊕ N)
+           by (unfold msub; now psimpl);
+           rewrite Theory_RISCV.getmem_mod_l with (a := (48 + N)) ||
+             rewrite Theory_RISCV.setmem_mod_l with (a := (48 + N))
+    end; (* the simpl calls aren't simplifying as intended... *) psimpl.
+
+
+Lemma noverlap_index_l:
+  forall w a1 len1 a2 len2 index size
+  (NO : ~ overlap w a1 len1 a2 len2)
+  (IN : index + size <= len1),
+  ~ overlap w (a1 + index) size a2 len2.
+Proof.
+  intros.
+  remember (a1 + index) as a1'. apply noverlap_shrink with (a1:=a1) (len1:=len1).
+  rewrite Heqa1'. rewrite add_msub_l.
+  apply N.le_trans with (m:=index+size). rewrite <-N.add_le_mono_r. apply N.Div0.mod_le.
+  assumption.
+  assumption.
+Qed.
+
+Lemma noverlap_index_r:
+  forall w a1 len1 a2 len2 index size
+  (NO : ~ overlap w a1 len1 a2 len2)
+  (IN : index + size <= len2),
+  ~ overlap w a1 len1 (a2+index) size.
+Proof.
+  intros. eapply noverlap_symmetry, noverlap_index_l;[
+    eapply noverlap_symmetry; eassumption
+  | eassumption ].
+Qed.
+
+Lemma noverlap_index_index:
+  forall w a1 len1 a2 len2 index1 size1 index2 size2
+  (NO  : ~ overlap w a1 len1 a2 len2)
+  (IN1 : index1 + size1 <= len1)
+  (IN2 : index2 + size2 <= len2),
+  ~ overlap w (a1 + index1) size1 (a2 + index2) size2.
+Proof.
+  intros. apply noverlap_index_l with (len1:=len1).
+  apply noverlap_symmetry. apply noverlap_index_l with (len1:=len2).
+  apply noverlap_symmetry.
+  all: assumption.
+Qed.
+
+
+Theorem _models_var:
+  forall v {c s} (MDL: models c s),
+  match c v with Some (NumT w) => 
+                  match s v with
+                  | VaN v _ => v < 2^w
+                  | _ => False
+                  end
+               | _ => True end.
+Proof.
+  intros. destruct (c v) eqn:CV; [|exact I].
+  specialize (MDL _ _ CV). inversion MDL; easy.
+Qed.
+
+Theorem models_var:
+  forall v {c s} (MDL: models c s) x w,
+  s v = VaN x w -> match c v with 
+                   | Some (NumT w) => x < 2^w 
+                   | _ => True 
+                   end.
+Proof.
+  intros. assert (H':=_models_var v MDL). rewrite H in *.
+  destruct (c v) eqn:CV.
+  destruct t.  assumption.
+  unfold models in *. specialize (MDL v _ CV).
+  inversion MDL; subst. rewrite H in *; discriminate.
+  easy.
+Qed.
+
+(** Eliminate the store by rewriting the expressions stored in registers and
+    inferring their bounds from the type context. *)
+Global Ltac elimstore :=
+  repeat
+   lazymatch goal with
+   | H:?s ?v = VaN ?x ?w, MDL:models ?typs ?s
+     |- _ =>
+         let Hyp := fresh "SBound" in
+         pose proof (models_var v MDL x w H) as Hyp;
+         let tHyp := type of Hyp in
+         cbv -[N.lt N.pow] in Hyp;
+         let tHyp := type of Hyp in
+          match type of Hyp with
+          | _ < 2 ^ ?w =>
+              assert (temp : (w <=? 256) = true) by reflexivity; clear temp
+          | _ => clear Hyp
+          end; try rewrite H in *; clear H; try clear s MDL
+   end.
+
+Global Ltac Zify.zify_pre_hook ::= elimstore; unfold msub in *.
+
+Module TimingProof (cpu: CPUTimingBehavior).
+
+Module Program_find_in_ll <: ProgramInformation.
     Definition entry_addr : N := 0x10250.
 
     Definition exits (t:trace) : bool :=
-    match t with (Addr a,_)::_ => match a with
-    | 0x102b8 => true
-    | _ => false
-  end | _ => false end.
-End find_in_linked_listTime.
+        match t with (Addr a,_)::_ => match a with
+        | 0x102b8 => true
+        | _ => false
+    end | _ => false end.
 
-Module find_in_linked_listAuto := TimingAutomation find_in_linked_listTime.
-Import find_in_linked_listTime find_in_linked_listAuto.
+    Definition binary := linked_list_bin.
+End Program_find_in_ll.
 
+Module RISCVTiming := RISCVTiming cpu Program_find_in_ll.
+Module find_in_ll := RISCVTimingAutomation RISCVTiming.
+Import Program_find_in_ll find_in_ll.
+
+Definition NULL : N := 0.
 Definition list_node_value (mem : addr -> N) (node : addr) : N :=
     mem Ⓓ[node].
 Definition list_node_next (mem : addr -> N) (node : addr) : N :=
-    mem Ⓓ[4 + node].
-Definition NULL : N := 0.
+  (* Original definition: mem Ⓓ[4 + node]. *)
+  (* Allowing NULL to have itself as the next node: *)
+  match node with 0 => NULL | _ => mem Ⓓ[4 + node] end.
 
 Inductive key_in_linked_list : (addr -> N) -> addr -> N -> nat -> Prop :=
 | KeyAtHead mem node key :
+    node <> NULL ->
     list_node_value mem node = key ->
     key_in_linked_list mem node key 0
 | KeyAtNext mem node key idx :
+    node <> NULL ->
+    list_node_value mem node <> key ->
     key_in_linked_list mem (list_node_next mem node) key idx ->
     key_in_linked_list mem node key (S idx).
 
 Fixpoint key_in_linked_list_dec (mem : addr -> N) (node : addr) (key : N) (idx : nat)
         : {key_in_linked_list mem node key idx} + {~ key_in_linked_list mem node key idx}.
+    destruct node as [|p];[|remember (Npos p) as node].
+    {
+      right. intro. dependent induction H; subst. contradiction.
+      assert (Help:list_node_next mem 0 ~= 0) by reflexivity.
+      now specialize (IHkey_in_linked_list Help).
+    }
+(* destruct (N.eq_dec (list_node_value mem node) key). *)
     destruct idx as [| idx'].
     - (* Base case: idx = 0 *)
         destruct (N.eq_dec (list_node_value mem node) key) as [Heq | Hneq].
-        + left. constructor. exact Heq.
+        + left. constructor. intro; now subst. assumption.
         + right. intros H. inversion H. subst. contradiction.
     - (* Inductive case: idx = S idx' *)
+        destruct (N.eq_dec (list_node_value mem node) key) as [Heq | Hneq].
+        { right; intro H; inversion H; contradiction. }
         destruct (key_in_linked_list_dec mem (list_node_next mem node) key idx') as [IN | NOT_IN].
-        + left. constructor. exact IN.
+        + left. constructor. intro; now subst. assumption. exact IN.
         + right. intros H. inversion H. subst. apply NOT_IN. assumption.
 Qed.
 
-Inductive well_formed_list : (addr -> N) -> addr -> list addr -> Prop :=
-| wf_nil : forall mem,
-    list_node_next mem NULL <> NULL ->
-    well_formed_list mem NULL []
-| wf_cons : forall mem n visited,
-    n <> NULL ->
-    list_node_next mem n <> n ->
-    (* next not in visited to avoid cycles *)
-    ~ In (list_node_next mem n) visited ->
-    well_formed_list mem (list_node_next mem n) (n :: visited) ->
-    well_formed_list mem n visited.
+(* node_in_linked_list allows for the looked up node to be NULL. *)
+Inductive node_in_linked_list : (addr -> N) -> addr -> addr -> Prop :=
+  | NodeAtHead : forall mem node, node_in_linked_list mem node node
+  | NodeInTail : forall mem node head
+    (NEQ: node <> head)
+    (NNUL: head <> NULL)
+    (IN: node_in_linked_list mem (list_node_next mem head) node),
+    node_in_linked_list mem head node.
 
-Inductive node_distance : addr -> addr -> nat -> Prop :=
-| Dst0 node :
-    node_distance node node 0
-| DstSn mem src dst len :
-    well_formed_list mem src [] ->
-    src <> dst ->
-    node_distance (list_node_next mem src) dst len ->
-    node_distance src dst (S len).
+(** A list is well formed if the head node points
+      1) NULL, or
+      2) the head of a well formed list. *)
+Inductive well_formed_list : (addr -> N) -> addr -> Prop :=
+| wf_nil : forall mem, well_formed_list mem NULL
+| wf_cons : forall mem n
+    (NNUL: n <> NULL)
+    (NEXTWF: well_formed_list mem (list_node_next mem n)),
+    well_formed_list mem n.
 
-Lemma well_formed_impl_next_neq_curr : forall mem src,
-    well_formed_list mem src [] ->
-    list_node_next mem src <> src.
+Inductive node_distance : (addr -> N) -> addr -> addr -> nat -> Prop :=
+| Dst0 : forall mem node,
+    node_distance mem node node 0
+| DstSn : forall mem src dst len
+    (NNUL: src <> NULL)
+    (NEQ: src <> dst)
+    (LEN: node_distance mem (list_node_next mem src) dst len),
+    node_distance mem src dst (S len).
+
+Theorem node_distance_uniq:
+  forall mem src dst len1 len2,
+    node_distance mem src dst len1 ->
+    node_distance mem src dst len2 ->
+    len1 = len2.
 Proof.
-    intros. induction H; subst.
+  intros mem src dst len1 len2 H; revert len2.
+  induction H; intros len2 L2.
+  - inversion L2; subst.
+      reflexivity.
+      contradiction.
+  - inversion L2; subst.
+      contradiction.
+      now rewrite (IHnode_distance len0).
+Qed.
+
+Theorem node_distance_uniq':
+  forall mem src dst1 len1 dst2 len2,
+    node_distance mem src dst1 len1 ->
+    node_distance mem src dst2 len2 ->
+    len1 = len2 -> dst1 = dst2.
+Proof.
+  intros mem src dst1 len1 dst2 len2 H; revert dst2 len2 .
+  induction H; intros dst2 len2 L2.
+  - inversion L2; subst.
+      reflexivity.
+      intro; discriminate.
+  - inversion L2; subst.
+      intro; discriminate.
+      intro EQ; injection EQ; clear EQ; intro EQ; subst len0.
+      eapply IHnode_distance; try eassumption. reflexivity.
+Qed.
+
+
+Theorem no_node_in_null:
+  forall mem node (NNUL: node <> NULL), ~node_in_linked_list mem NULL node.
+Proof.
+  intros; intro H; inversion H; subst; try contradiction.
+Qed.
+
+Theorem wf_has_null:
+  forall mem head (WF: well_formed_list mem head),
+  node_in_linked_list mem head NULL.
+Proof.
+  intros. induction WF.
+    constructor.
+    eapply NodeInTail; try easy.
+Qed.
+
+Theorem has_null_wf:
+  forall mem head (NUL: node_in_linked_list mem head NULL),
+  well_formed_list mem head.
+Proof.
+  intros. dependent induction NUL.
+    constructor.
+    eapply wf_cons; try easy.
+    apply IHNUL; reflexivity.
+Qed.
+
+Theorem well_formed_impl_next_not_same:
+  forall mem src (WF: well_formed_list mem src),
+  src = NULL \/ list_node_next mem src <> src.
+Proof.
+  intros.
+  destruct (N.eq_dec src NULL).
+    now left.
+    (* Interesting that inversion isn't enough, needed induction. *)
+    induction WF; subst; right.
+       contradiction.
+       intro H1; rewrite H1 in *. destruct (IHWF n).
+         subst; contradiction.
+         contradiction.
+Qed.
+
+Theorem only_null_in_null:
+  forall mem node,  node_in_linked_list mem NULL node -> node = NULL.
+Proof.
+  intros mem node H. inversion H; subst; try easy.
+Qed.
+
+Theorem in_impl_next_in:
+  forall mem n n' head
+    (NEXT: n' = list_node_next mem n)
+    (IN: node_in_linked_list mem head n),
+  node_in_linked_list mem head n'.
+Proof.
+  intros. revert NEXT; revert n'.
+  dependent induction IN.
+  - intros. destruct (N.eq_dec node NULL);[subst node|].
+      cbn in NEXT; subst; constructor.
+      destruct (N.eq_dec n' node) as [e|e];[subst n';rewrite e in *; constructor|].
+      apply NodeInTail; try easy. rewrite <-NEXT; constructor.
+  - rename IHIN into IH. intros. remember (list_node_next mem head) as head'. move n' before node.
+    specialize (IH _ NEXT).
+    destruct (N.eq_dec n' head) as [e|e];[rewrite e; apply NodeAtHead|].
+    apply NodeInTail; try easy. rewrite <-Heqhead'; assumption.
+Qed.
+
+Theorem well_formed_impl_not_in_strong:
+  forall mem src (NNUL: src <> NULL) (WF: well_formed_list mem src),
+  forall node (IN: node_in_linked_list mem src node),
+  ~node_in_linked_list mem (list_node_next mem node) src.
+Proof.
+  intros mem src NNUL WF. dependent induction WF generalizing NNUL. intros node IN.
+  - contradiction.
+  - remember (list_node_next mem n) as n'. clear NNUL0.
+    (* n -> n' ... *)
+    destruct (N.eq_dec n' NULL).
+    (* next node, node, is null, reached end of list without finding src *)
+    (* n -> NULL = n'*)
+    + intros node IN IN2. subst n'.
+      (* Node must be NULL or n, we prove a contradiction in either case. *)
+      assert (CASE: node = NULL \/ node = n).
+      inversion IN; subst.
+        right; reflexivity.
+        destruct (N.eq_dec node NULL);[left; assumption|rewrite e in *]. now assert (H':=only_null_in_null _ _ IN0).
+      destruct CASE.
+        (* node is NULL *)
+        subst node. inversion IN; subst; try easy. rewrite e in *; clear e IHWF NNUL NNUL0. 
+        cbn in IN2; apply only_null_in_null in IN2. symmetry in IN2; contradiction.
+        (* node is n *)
+        subst node. rewrite e in *. apply only_null_in_null in IN2; contradiction.
+    (* n -> n' -> ... -> node -> node' -> ... *)
+    + intros node IN In2; remember (list_node_next mem node) as node'; rename IHWF into IH;
+      specialize (IH n0); rename In2 into IN2.
+      (* WF n'
+         def: node -> node'
+         IN: n -> ... -> node
+         In2: node' -> ... -> n
+         IH: (n' ~~> ?x) -> (~ ?x' ~~> n')
+         So say ?x is node. If node is n we have a cycle, otherwise use IH.
+      *)
+      move IN before IN2. move IH before IN. move Heqnode' after Heqn'.
+      specialize (IH node).
+      inversion IN;[subst node0 node mem0|].
+        rewrite <-Heqn' in *; subst node'; specialize (IH IN2); apply IH; constructor.
+        subst mem0 node0 head; rewrite <-Heqn' in *; specialize (IH IN0); rewrite <-Heqnode' in *.
+        move NEQ before n0; clear NNUL0.
+        assert (CONTRA:=in_impl_next_in _ _ _ _ Heqn' IN2); contradiction.
+Qed.
+
+Theorem well_formed_impl_not_in:
+  forall mem src (NNUL: src <> NULL) (WF: well_formed_list mem src),
+  ~node_in_linked_list mem (list_node_next mem src) src.
+Proof.
+  intros. eapply (well_formed_impl_not_in_strong _ _ _ _ _). Unshelve.
+  constructor.
+  all:assumption.
+Qed.
+
+Lemma well_formed_impl_next_neq_curr : 
+  forall mem src
+    (NNUL: src <> NULL)
+    (WF: well_formed_list mem src),
+  list_node_next mem src <> src.
+Proof.
+    intros. induction WF; subst.
         assumption.
-    intro. rewrite H3 in *. contradiction.
+    intro. rewrite H in *. specialize (IHWF NNUL0). contradiction.
 Qed.    
 
-Lemma node_distance_len_nonzero : forall head len,
-    node_distance head NULL len ->
+Lemma node_distance_len_nonzero : forall m head len,
+    node_distance m head NULL len ->
     negb (head =? NULL) = true ->
     (0 < len)%nat.
 Proof.
@@ -87,59 +394,748 @@ Proof.
     lia.
 Qed.
 
-Lemma node_distance_same : forall h n,
-    node_distance h h n -> n = O.
+Lemma node_distance_same : forall m h n,
+    node_distance m h h n -> n = O.
 Proof.
     intros. inversion H; subst. reflexivity.
     contradiction.
 Qed.
 
-Lemma node_distance_null_dupe : forall head tail n1 n2,
-    node_distance head tail n1 ->
-    node_distance head tail n2 ->
+Ltac gdep n := generalize dependent n.
+Lemma node_distance_null_dupe : forall m head tail n1 n2,
+    node_distance m head tail n1 ->
+    node_distance m head tail n2 ->
     n1 = n2.
-Abort.
-    
+Proof.
+  intros m head tail n1. gdep head; gdep tail.
+  induction n1 as [n1 IHn1] using lt_wf_ind.
+  intros tail head n2 N1 N2.
+  inversion N1; subst.
+    now inversion N2.
+    inversion N2; subst.
+      contradiction.
+      specialize (IHn1 len (Nat.lt_succ_diag_r _) _ _ len0 LEN LEN0). now subst.
+Qed.
 
+(* Inductive type for properties holding for all nodes in a list.
+   The property P is a function from memory and address to a prop. *)
+Inductive LLForall (P: (addr->N)->N->Prop): (addr -> N) -> N -> Prop :=
+  | LLForall_nil : forall mem, LLForall P mem NULL
+  | LLForall_cons : forall mem addr 
+                      (NNUL: addr <> NULL) 
+                      (HEAD: P mem addr) 
+                      (TAIL: LLForall P mem (list_node_next mem addr)),
+                    LLForall P mem addr.
+
+(* Specify a loose bound on the minimum address of nodes in a linked list.
+   This doesn't guarantee any node actually has this address. *)
+Definition LLBounds mem addr min max := LLForall (fun _ a => min <= a <= max) mem addr.
+Inductive LLSame : (addr->N) -> (addr->N) -> N -> Prop :=
+  | LLSame_nil : forall mem mem', LLSame mem mem' NULL
+  | LLSame_cons : forall mem mem' head,
+                  (list_node_value mem head) = (list_node_value mem' head) ->
+                  (list_node_next mem head) = (list_node_next mem' head) ->
+                  LLSame mem mem' (list_node_next mem head) ->
+                  LLSame mem mem' head.
+
+Theorem llsame_ind:
+  forall mem head (f:(addr->N)->(addr->N))
+    (PRES:LLForall (fun mem' a => list_node_value mem a = list_node_value mem' a /\ list_node_next mem a = list_node_next mem' a)
+      (f mem) head),
+  LLSame mem (f mem) head.
+Proof.
+  intros. dependent induction PRES;[constructor|].
+  destruct HEAD as [Val Next].
+  apply LLSame_cons; try easy; rename addr into a.
+  specialize (IHPRES mem f (eq_refl _) (eq_refl _)).
+  now rewrite Next.
+Qed.
+
+Theorem noverlap_llsame:
+  forall mem e wraddr wrlen v head min max
+    (LLB: LLBounds mem head min max)
+    (NOV: ~overlap 32 wraddr wrlen min (max+8-min)),
+  LLSame mem (setmem 32 e wrlen mem wraddr v) head.
+Proof.
+  intros. pose (fun mem => setmem 32 e wrlen mem wraddr v) as f.
+  replace (setmem _ _ _ _ _ _) with (f mem); try reflexivity.
+  apply llsame_ind.
+  dependent induction LLB.
+  { apply LLForall_nil. }
+  {
+    rename addr into a.
+    assert (Rem:list_node_next mem a = list_node_next (f mem) a).
+    (* noverlap_sum + lia can't handle this either *)
+    { destruct a as [|p];[contradiction|].
+      unfold f, list_node_next; rewrite getmem_noverlap;[reflexivity|].
+      apply noverlap_symmetry; remember (N.pos p) as a.
+      pose (4 + a - min) as i. replace (4+a) with (min+i) by lia.
+      eapply noverlap_index_r. exact NOV. lia.
+    }
+    assert (Rem2:list_node_value mem a = list_node_value (f mem) a).
+    (* noverlap_sum + lia can't handle this either *)
+    { destruct a as [|p];[contradiction|].
+      unfold f, list_node_value; rewrite getmem_noverlap;[reflexivity|].
+      apply noverlap_symmetry; remember (N.pos p) as a.
+      pose (a - min) as i. replace (a) with (min+i) by lia.
+      eapply noverlap_index_r. exact NOV. lia.
+    }
+    apply LLForall_cons; try easy.
+    specialize (IHLLB NOV).
+    unfold f at 1. rewrite <-Rem.
+    apply IHLLB.
+  }
+Qed.
+
+Theorem llforall_next:
+  forall mem head p
+    (ALL: LLForall p mem head),
+  LLForall p mem (list_node_next mem head).
+Proof.
+  intros. dependent induction ALL;[simpl;constructor|assumption].
+Qed.
+
+Theorem llbounds_next:
+  forall mem head min max, LLBounds mem head min max -> LLBounds mem (list_node_next mem head) min max.
+Proof.
+  intros. now apply llforall_next.
+Qed.
+
+Theorem noverlap_llsame_trans:
+  forall mem mem' e wraddr wrlen v head min max
+    (LLB: LLBounds mem head min max)
+    (LLS: LLSame mem mem' head)
+    (NOV: ~overlap 32 wraddr wrlen min (max+8-min)),
+    LLSame mem (setmem 32 e wrlen mem' wraddr v) head.
+Proof.
+  intros. dependent induction LLS;[constructor|].
+  rename IHLLS into IH, H into VAL, H0 into NEXT; move mem' before mem.
+  specialize (IH (llbounds_next _ _ _ _ LLB) NOV).
+  destruct LLB; [constructor|].
+  destruct HEAD as [LO HI]; clear LLB. constructor. 3: exact IH.
+  unfold list_node_value. rewrite getmem_noverlap. now unfold list_node_value in VAL.
+  (* Interesting, lia doesn't work for this noverlap goal, so have to do it logically... *)
+  pose (addr-min) as i.
+  replace addr with (min+i) by lia.
+  eapply noverlap_index_l. apply noverlap_symmetry; eassumption. lia.
+
+  clear - LO HI NEXT NNUL NOV; unfold list_node_next in *.
+  destruct addr;[contradiction|remember (N.pos p) as addr].
+  rewrite getmem_noverlap; try easy.
+  pose (addr - min) as i. replace (4+addr) with (min+(i+4)) by lia. apply noverlap_symmetry.
+  eapply noverlap_index_r; try eassumption; try lia.
+Qed.
+
+Theorem LLForall_ind':
+  forall P mem head,
+    P mem head ->
+    (forall n, node_in_linked_list mem head n -> P mem n) ->
+    LLForall P mem head.
+Proof.
+  intros. destruct head; constructor.
+  easy. easy.
+Abort.
+
+
+(*
+Theorem LLSame_ind' : 
+       ()
+       (forall mem mem' : addr -> N, LLSame mem mem' NULL) ->
+       (forall (mem mem' : addr -> N) (head : addr),
+        head <> NULL ->
+        list_node_value mem head = list_node_value mem' head ->
+        list_node_next mem head = list_node_next mem' head ->
+        LLSame mem mem' (list_node_next mem head) ->
+        LLSame mem mem' (list_node_next mem head) -> LLSame mem mem' head) ->
+       forall (n n0 : addr -> N) (n1 : N), LLSame n n0 n1.
+Proof.
+  intros. destruct n1.
+  constructor.
+  apply H0; try easy.
+ *)
+
+
+
+Theorem llsame_same:
+  forall mem head len, node_distance mem head NULL len -> LLSame mem mem head.
+Proof.
+  intros m head len LEN. dependent induction LEN;[constructor|].
+  specialize (IHLEN (JMeq_refl 0)).
+  constructor; try easy.
+Qed.
+
+Theorem llsame_same':
+  forall mem head, LLSame mem mem head.
+Proof.
+  intros m head. constructor; try easy.
+  (* Now what?? *)
+Abort.
+
+Theorem llsame_bounds:
+  forall mem mem' head min max
+    (SAME: LLSame mem mem' head)
+    (LLB: LLBounds mem head min max),
+  LLBounds mem' head min max.
+Proof.
+  unfold LLBounds; intros. revert SAME; revert mem'.
+  dependent induction LLB.
+    constructor.
+    intros; inversion SAME; subst.
+      contradiction.
+      constructor; try easy.
+      rewrite <-H0. now apply IHLLB.
+Qed.
+
+Theorem llsame_distance:
+  forall mem mem' head node len
+    (SAME:LLSame mem mem' head)
+    (LEN: node_distance mem head node len),
+  node_distance mem' head node len.
+Proof.
+  intros. dependent induction LEN;[constructor|].
+  constructor; try easy.
+  inversion SAME;subst;[contradiction|].
+  rewrite <-H0. now apply IHLEN.
+Qed.
+
+Theorem llsame_symmetry:
+  forall ml mr h, LLSame ml mr h <-> LLSame mr ml h.
+Proof.
+  intros; split; intro H; induction H; subst.
+  1,3:apply LLSame_nil.
+  all:apply LLSame_cons; try easy; now rewrite H0 in IHLLSame.
+Qed.
+
+(* Conveniently saves us a book-keeping clause in the loop invariant stating
+   the current node is not null. *)
+Theorem dist_lt_null_not_null:
+  forall mem head node nodelen dst dstlen
+    (NODE: node_distance mem head node nodelen)
+    (DST: node_distance mem head dst dstlen)
+    (LT: (nodelen < dstlen)%nat),
+  node <> dst.
+Proof.
+  intros. gdep LT; gdep nodelen; gdep node. dependent induction DST;[lia|].
+  intros.
+  assert (H: N : Type) by constructor.
+  Local Ltac mvvars T :=
+    assert (Temp: N : Type) by constructor;
+    idtac "Collecting vars of " T; clear Temp;
+    repeat match goal with
+    | [vtop: T |- _] =>
+        idtac "vtop: " vtop;
+        repeat match goal with 
+        | [v: T |- _] => idtac "v: " v "vtop: " vtop; first [
+              idtac "in first"; fail 0
+            | assert (Temp: vtop = v) by reflexivity; clear Temp (* don't move the same var *)
+            | move v before vtop ]
+        end end.
+  mvvars nat.
+
+
+  move node before len; move nodelen before len; move NODE before DST;  rename IHDST into IH.
+  inversion NODE; subst; try assumption.
+  eapply IH; clear IH NNUL0; move len0 before len; move NEQ0 before NEQ; move LT after LEN; unfold lt in LT.
+  eassumption.
+  lia.
+Qed.
+
+Theorem distance_imp_head_next_nnul:
+  forall mem head dst len'
+    (DST: dst <> NULL)
+    (LEN: node_distance mem head dst (S len')),
+  list_node_next mem head <> NULL.
+Proof.
+  intros. inversion LEN; subst. inversion LEN0; subst; try easy.
+Qed.
+
+Theorem distance_imp_in:
+  forall mem head dst len,
+    node_distance mem head dst len -> node_in_linked_list mem head dst.
+Proof.
+  intros. dependent induction H;[constructor|rename IHnode_distance into IH].
+  constructor; try easy.
+Qed.
+
+Theorem next_node_in_linked_list:
+  forall mem head n, n <> NULL -> node_in_linked_list mem head n -> node_in_linked_list mem head (list_node_next mem n).
+Proof.
+  intros. induction H0.
+    destruct (N.eq_dec (list_node_next mem node) node) as [EQ|NEQ];[rewrite EQ in *|]; constructor; try easy; constructor.
+    rename IHnode_in_linked_list into IH. remember (list_node_next mem node) as next. specialize (IH H).
+    inversion IH; subst mem0 node0; try subst head0.
+      - clear - NNUL. destruct (N.eq_dec head (list_node_next mem head)) as [Eq|?];[rewrite Eq at 1; apply NodeAtHead|].
+        apply NodeInTail; try easy. apply NodeAtHead.
+      - destruct (N.eq_dec next head);[| apply NodeInTail; try easy].
+        subst head. apply NodeAtHead.
+Qed.
+
+Theorem in_well_formed_imp_well_formed:
+  forall mem head node
+    (WF: well_formed_list mem head)
+    (IN: node_in_linked_list mem head node),
+  well_formed_list mem node.
+Proof.
+  intros. dependent induction IN;[assumption|].
+  apply IHIN. inversion WF; subst;[contradiction|assumption].
+Qed.
+
+(* This is not generally true for lists with cycles. Observe the difference between
+   the distances of X and Y, and X' and Y' below:
+
+            X -> X' -> Y' -> _ -> _ -> _ -> Y
+                        ^--------------------+ 
+*)
+Theorem node_distance_next_next_same:
+  forall mem head (dst:addr) len
+    (NNUL: dst <> NULL)
+    (WF: well_formed_list mem head)
+    (LEN: node_distance mem head dst len),
+  node_distance mem (list_node_next mem head) (list_node_next mem dst) len.
+Proof.
+  intros mem head dst len. gdep dst; gdep head; gdep mem. induction len.
+  {
+    intros. inversion LEN; subst; constructor.
+  }
+  {
+    intros. rename IHlen into IH.
+    destruct (N.eq_dec head NULL);[inversion LEN; now subst|].
+    apply DstSn; try easy. 
+    - (* contradiction if head->null because there's distance between head and dst, and dst is not null. *)
+      eapply distance_imp_head_next_nnul with (dst:=dst); try eassumption.
+    - clear - NNUL n WF LEN. intro. inversion WF; subst; try easy. 
+      clear n; move NNUL0 after NNUL.
+      assert (Help:=distance_imp_in _ _ _ _ LEN).
+      inversion Help; subst.
+      + inversion LEN; now subst.
+      + rewrite H in IN. apply (in_well_formed_imp_well_formed _ _ _ WF) in Help.
+        apply (well_formed_impl_not_in _ _ NNUL Help). assumption.
+    - apply IH; try easy. inversion WF; subst; try easy.
+      inversion LEN; subst; try easy.
+  }
+Qed.
+
+Theorem next_node_is_in:
+  forall mem node
+    (NNUL: node <> NULL),
+  node_in_linked_list mem node (list_node_next mem node).
+Proof.
+  intros. destruct (N.eq_dec (list_node_next mem node) node).
+  - rewrite e; constructor.
+  - constructor; try easy. constructor.
+Qed.
+
+Theorem wf_imp_next_diff:
+  forall mem node, node <> NULL -> well_formed_list mem node -> list_node_next mem node <> node.
+Proof.
+  intros mem node NNUL WF. intro. inversion WF; subst; try easy.
+  assert (Help:=well_formed_impl_not_in _ _ NNUL WF).
+  assert (Help2:=next_node_is_in mem _ NNUL). rewrite H in Help2. rewrite <-H in Help2 at 1. contradiction.
+Qed.
+
+(* This is not generally true of lists with cycle, Consider the situation below:
+
+      head -> dst' -> _ -> _ -> dst 
+               ^-----------------+
+*)
+Theorem node_distance_next_S_len:
+  forall mem head dst len
+    (NNUL: dst <> NULL)
+    (WF: well_formed_list mem head)
+    (LEN: node_distance mem head dst len),
+  node_distance mem head (list_node_next mem dst) (S len).
+Proof.
+  intros. destruct (N.eq_dec head NULL);[inversion LEN; subst; contradiction|].
+  {
+    destruct len. inversion LEN; subst. constructor; try easy.
+    symmetry; apply wf_imp_next_diff; try easy.
+    constructor.
+    constructor; try easy.
+    (* Well-formedness contradiction subproof. *)
+    { intro.
+      assert (Help:=distance_imp_in _ _ _ _ LEN).
+      assert (WFDST:=in_well_formed_imp_well_formed _ _ _ WF Help).
+      move n after NNUL; move WF before WFDST; move H after LEN.
+      assert (Help3:=well_formed_impl_not_in _ _ NNUL WFDST).
+      now rewrite H in Help.
+    }
+    apply node_distance_next_next_same; try easy.
+  }
+Qed.
+
+Theorem distance_null_imp_well_formed:
+  forall mem head len
+    (LEN: node_distance mem head NULL len),
+  well_formed_list mem head.
+Proof.
+  intros. dependent induction LEN;[constructor|].
+  rename IHLEN into IH; assert (Help:0~=NULL) by reflexivity; specialize (IH Help); clear Help NEQ.
+  apply wf_cons; try easy.
+Qed.
+  
+Theorem distance_imp_diff:
+  forall mem head n len
+    (LEN: node_distance mem head n (S len)),
+  head <> n.
+Proof.
+  intros. intro. inversion LEN; subst. contradiction.
+Qed.
+
+Theorem wf_by_parts:
+  forall mem head n len
+    (WFTail: well_formed_list mem n)
+    (LEN: node_distance mem head n len),
+  well_formed_list mem head.
+Proof.
+  intros. dependent induction LEN;[assumption|].
+  specialize (IHLEN WFTail). constructor; try easy.
+Qed.
+
+Theorem distance_last_node:
+  forall mem head n len
+    (NNUL: n <> NULL)
+    (LEN: node_distance mem head n len)
+    (NIL: list_node_next mem n = NULL),
+  node_distance mem head NULL (S len).
+Proof.
+  intros. rewrite <-NIL.
+  apply node_distance_next_S_len; try easy.
+  eapply wf_by_parts; try eassumption.
+  constructor; try easy.
+  rewrite NIL; constructor.
+Qed.
+
+Theorem node_in_linked_list_trans:
+  forall mem head m dst
+    (IN1: node_in_linked_list mem head m)
+    (IN2: node_in_linked_list mem m dst),
+  node_in_linked_list mem head dst.
+Proof.
+  intros mem head m dst IN1; gdep dst; dependent induction IN1;[now intros|].
+  intros. destruct (N.eq_dec dst head);[subst dst; constructor|].
+  constructor; try easy.
+  now apply IHIN1.
+Qed.
+
+Theorem node_distance_split:
+  forall mem head m dst pre post
+    (WF: well_formed_list mem head)
+    (PRE: node_distance mem head m (pre))
+    (POST: node_distance mem m dst post),
+  node_distance mem head dst (pre+post)%nat.
+Proof.
+  intros mem head m dst pre post WF PRE. gdep WF; gdep dst; gdep post. dependent induction PRE;[now simpl|].
+  rename len into pre'; rename src into head; rename dst into m.
+  intros post dst WF POST. move post before pre'; move dst before m.
+  rewrite Nat.add_succ_l. destruct (N.eq_dec head dst).
+  {
+    subst dst. exfalso. 
+    eapply well_formed_impl_not_in; try eassumption.
+    assert (IN1:=distance_imp_in _ _ _ _ PRE);
+    assert (IN2:=distance_imp_in _ _ _ _ POST).
+    apply node_in_linked_list_trans with (m:=m); try easy.
+  }
+  {
+    apply DstSn; try easy.
+    apply IHPRE; try easy.
+    inversion WF; subst; try easy.
+  }
+Qed.
+
+Theorem key_loc_split:
+  forall mem head node key pre post
+    (DIST: node_distance mem head node (pre))
+    (KEY: key_in_linked_list mem head key (pre+post)),
+  key_in_linked_list mem node key post.
+Proof.
+  intros mem head node key pre post DIST. dependent induction DIST;[now simpl|].
+  intros. inversion KEY; subst.
+  specialize (IHDIST H5). assumption.
+Qed.
+
+Theorem no_key_in_null:
+  forall mem key len, ~key_in_linked_list mem NULL key len.
+Proof. 
+  intros. intro H. dependent induction H; subst. contradiction.
+  assert (Help:list_node_next mem 0 ~= NULL) by reflexivity.
+  now specialize (IHkey_in_linked_list Help).
+Qed.
+
+
+Theorem key_loc_lt_length:
+  forall mem head len key loc
+    (LEN: node_distance mem head NULL len)
+    (LOC: key_in_linked_list mem head key loc),
+  (loc < len)%nat.
+Proof.
+  intros. move loc after len. destruct (Nat.lt_ge_cases loc len) as [Lt | Ge];[assumption|exfalso].
+  pose (loc-len)%nat as post.
+  replace loc with (len+post)%nat in LOC by lia.
+  apply (key_loc_split _ _ _ _ _ _ LEN) in LOC.
+  now apply no_key_in_null in LOC.
+Qed.
+
+Theorem key_loc_le_instance:
+  forall mem head key loc1 node loc2
+    (LEN: node_distance mem head node loc2)
+    (INST: list_node_value mem node = key)
+    (LOC: key_in_linked_list mem head key loc1),
+  (loc1 <= loc2)%nat.
+Proof.
+  intros. move loc2 before loc1; move node before head. destruct (Nat.le_gt_cases loc1 loc2) as [Le | Gt];[assumption|exfalso].
+  pose (loc1-loc2)%nat as post.
+  replace loc1 with (loc2+post)%nat in LOC by lia.
+  apply (key_loc_split _ _ _ _ _ _ LEN) in LOC.
+  inversion LOC;[lia|].
+  subst mem0 node0 key0.
+  contradiction.
+Qed.
+
+
+Theorem key_in_linked_list_value_equal:
+  forall mem head key loc node
+    (Key: key_in_linked_list mem head key loc)
+    (Dist: node_distance mem head node loc),
+  key = list_node_value mem node.
+Proof.
+  intros mem head key loc node Key; gdep node. dependent induction Key.
+  {
+    intros. inversion Dist; subst. reflexivity.
+  }
+  {
+    intros. rename node0 into kn. apply IHKey.
+    inversion Dist; now subst.
+  }
+Qed.
+
+Theorem fuel_le_incr:
+  forall mem head key curr ctr
+    (Ctr:node_distance mem head curr ctr)
+    (Fuel:forall fuel, key_in_linked_list mem head key fuel -> (ctr <= fuel)%nat)
+    (BC: key <> list_node_value mem curr),
+  forall fuel, key_in_linked_list mem head key fuel -> (S ctr <= fuel)%nat.
+Proof.
+  intros. specialize (Fuel _ H). destruct (Nat.lt_ge_cases ctr fuel);[lia|exfalso].
+  assert (Help:fuel=ctr) by lia; rewrite Help in *; clear Fuel H0 Help.
+  assert (Contra:=key_in_linked_list_value_equal _ _ _ _ _ H Ctr).
+  contradiction.
+Qed.
+
+Theorem node_in_tail:
+  forall mem head n
+    (IN:node_in_linked_list mem head n)
+    (NNUL:head <> NULL)
+    (NEQ:head <> n),
+  node_in_linked_list mem (list_node_next mem head) n.
+Proof.
+  intros. dependent induction IN.
+  contradiction.
+  assumption.
+Qed.
+
+Theorem llsame_value:
+  forall mem mem' head node v
+    (IN: node_in_linked_list mem head node)
+    (LLS: LLSame mem mem' head)
+    (V: list_node_value mem node = v)
+    (NNUL: node <> NULL),
+  list_node_value mem' node = v.
+Proof.
+  intros. gdep V; gdep IN; gdep node. dependent induction LLS; intros.
+  - inversion IN; now subst.
+  - destruct (N.eq_dec head NULL);[subst; now inversion IN|].
+    destruct (N.eq_dec head node);[subst; now inversion IN|].
+    assert (H1:=node_in_tail _ _ _ IN n n0).
+    apply IHLLS; try easy.
+Qed.
+
+Theorem llsame_node_in:
+  forall mem mem' head node
+    (IN: node_in_linked_list mem head node)
+    (LLS: LLSame mem mem' head),
+  node_in_linked_list mem' head node.
+Proof.
+  intros. gdep IN; gdep node. dependent induction LLS; intros.
+  - inversion IN; subst. apply NodeAtHead. contradiction.
+  - move node before head.
+    destruct (N.eq_dec head NULL). subst; assert (t:=only_null_in_null _ _ IN); subst; constructor.
+    destruct (N.eq_dec head node). subst; constructor.
+    apply NodeInTail; try easy. rewrite <-H0; apply IHLLS. inversion IN;[subst; contradiction|assumption].
+Qed.
+
+Theorem llsame_value_neq:
+  forall mem mem' head node v
+    (IN: node_in_linked_list mem head node)
+    (LLS: LLSame mem mem' head)
+    (V: list_node_value mem node <> v)
+    (NNUL: node <> NULL),
+  list_node_value mem' node <> v.
+Proof.
+  intros. intro. 
+  apply llsame_node_in with (mem':=mem') in IN; try assumption.
+  rewrite llsame_symmetry in LLS.
+  assert(Help:=llsame_value _ _ _ _ _ IN LLS H NNUL).
+  contradiction.
+Qed.
+
+Theorem llsame_next_node:
+  forall mem mem' head node
+    (IN: node_in_linked_list mem head node)
+    (LLS: LLSame mem mem' head)
+    (NNUL: node <> NULL),
+  list_node_next mem node = list_node_next mem' node.
+Proof.
+  intros. gdep IN; dependent induction LLS; intro.
+  - eassert (H:=only_null_in_null _ _ IN). contradiction.
+  - destruct (N.eq_dec head NULL). subst; assert (t:=only_null_in_null _ _ IN); subst; constructor.
+    destruct (N.eq_dec head node). subst. assumption.
+    apply IHLLS; try easy.
+    now apply node_in_tail.
+Qed.
+
+Theorem llsame_key_in:
+  forall mem mem' head key loc
+    (Key: key_in_linked_list mem head key loc)
+    (LLS: LLSame mem mem' head),
+  key_in_linked_list mem' head key loc.
+Proof.
+  intros mem mem' head key loc Key; gdep mem'; dependent induction Key.
+  { intros. constructor; try easy. inversion LLS; now subst. }
+  rename IHKey into IH.
+  intros. move mem' before mem.
+  apply KeyAtNext. assumption.
+  replace (list_node_next mem' node) with (list_node_next mem node) by (inversion LLS; now subst).
+  eapply llsame_value_neq; try eassumption. constructor.
+  erewrite llsame_next_node with (mem':=mem); try eassumption.
+  apply IH.
+  inversion LLS; subst.
+    simpl; constructor.
+    assumption.
+  eapply llsame_node_in; try eassumption. constructor.
+  apply llsame_symmetry. assumption.
+Qed.
+
+Theorem noverlap_llbounds_shrink:
+  forall mem head min max node w a2 len2
+    (NNUL: node <> NULL)
+    (LLB: LLBounds mem head min max)
+    (IN: node_in_linked_list mem head node)
+    (NOV: ~overlap w min (8+max) a2 len2),
+  ~overlap w node 8 a2 len2.
+Proof.
+  intros. dependent induction IN; rename node into addr.
+  inversion LLB; subst;[contradiction|].
+  pose (addr-min) as i.
+  replace addr with (min+i) by lia.
+  eapply noverlap_index_l. eassumption. lia.
+
+  inversion LLB; subst;[contradiction|]. apply IHIN; try easy.
+Qed.
+
+Theorem key_not_in_list:
+  forall mem head key n nloc
+    (NNUL: n <> NULL)
+    (LAST: list_node_next mem n = NULL)
+    (NLOC: node_distance mem head n nloc)
+    (KLOC: forall kloc, key_in_linked_list mem head key kloc -> (nloc <= kloc)%nat)
+    (NEQ: list_node_value mem n <> key),
+  forall kloc, ~key_in_linked_list mem head key kloc.
+Proof.
+  intros. intro H. specialize (KLOC _ H).
+  assert (H2:node_distance mem head NULL (S nloc)).
+  {
+    inversion H; subst.
+    - rewrite <-Nat.add_1_r. apply node_distance_split with (m:=n); try easy.
+      apply has_null_wf, node_in_linked_list_trans with (m:=n).
+      eapply distance_imp_in; eassumption.
+      1-2: constructor; try easy; rewrite LAST; constructor.
+    - rewrite <-Nat.add_1_r. apply node_distance_split with (m:=n); try easy.
+      apply has_null_wf, node_in_linked_list_trans with (m:=n).
+      eapply distance_imp_in; eassumption.
+      1-2: constructor; try easy; rewrite LAST; constructor.
+  }
+  assert (H3:=key_loc_lt_length _ _ _ _ _ H2 H).
+  assert (H4:nloc = kloc) by lia; subst kloc; clear KLOC H3.
+  assert (H5:=key_in_linked_list_value_equal _ _ _ _ _ H NLOC); symmetry in H5.
+  contradiction.
+Qed.
+
+(* This is only true because the location of key is not unique,
+  will have to change our reasoning for the key-found in linked list
+  postcondition after changing the key_in_linked_list def. *)
+Theorem key_at_node:
+  forall mem head key node loc
+    (Dist: node_distance mem head node loc)
+    (NNul: node <> NULL)
+    (Key: list_node_value mem node = key)
+    (Min: forall i, key_in_linked_list mem head key i -> (loc <= i)%nat),
+  key_in_linked_list mem head key loc.
+Proof.
+  intros mem head key node loc Dist; dependent induction Dist; intros.
+  { constructor; try easy. }
+  assert (NEQk: list_node_value mem src <> key). {
+    intro.
+    destruct (key_in_linked_list_dec mem src key 0). specialize (Min _ k); lia.
+    apply n; constructor; try easy.
+  }
+  apply KeyAtNext; try easy.
+  apply IHDist; try easy.
+  intros.
+  enough (H1:key_in_linked_list mem src key (S i)).
+  specialize (Min (S i) H1); lia.
+  apply KeyAtNext; try easy.
+Qed.
+  
 Definition time_of_find_in_linked_list (mem : addr -> N) 
-        (head : addr) (key : N) (len : nat) (found_idx : option N)
+        (head : addr) (key : N) (len : nat) (found_idx : option nat)
         (t : trace) :=
     cycle_count_of_trace t =
         (* setup time *)
-        2 + 2 * time_mem + 2 + 3 * time_mem +
+        taddi + 2 * tsw + taddi + 2 * tsw + tlw +
         if head =? NULL then
-            3 + 2 + time_branch + 2 + 2 * time_mem + 2 + time_branch
+            tfbne + taddi + tjal + taddi + 2 * tlw + taddi + tjalr
         else (
-            time_branch + time_mem + time_branch +
-            (match found_idx with None => N.of_nat len | Some idx => idx end) *
-            (3 * time_mem + time_branch + 4 * time_mem + time_branch)
+        (* added: *)
+        match found_idx with
+        | None => 
+            tjalr + taddi + tlw + tlw + taddi + tlw + tfbne + tlw + tlw + tlw + tlw + tlw + taddi + ttbne + tsw
+        | Some _ =>
+            tjalr + taddi + tlw + tlw + taddi + tjal + tlw + tfbne + tlw + tlw + tlw
+        end +
+        (* added^ *)
+            ttbne + tlw + ttbne +
+            (N.of_nat match found_idx with None => Nat.pred len | Some idx => idx end) *
+            (3 * tlw + ttbne + 3 * tlw + tsw + ttbne)
         ).
 
-Definition timing_postcondition (mem : addr -> N) (head : addr)
-        (key : N) (t : trace) : Prop :=
-    exists len, node_distance head NULL len /\
-    time_of_find_in_linked_list mem head key len None t.
 
 Definition find_in_linked_list_timing_invs (s : store) (base_mem : addr -> N)
     (sp : N) (head : addr) (key : N) (len : nat) (t:trace) : option Prop :=
 match t with (Addr a, s) :: t' => match a with
 | 0x10250 => Some (s V_MEM32 = Ⓜbase_mem /\ s R_SP = Ⓓsp /\
-    s R_A0 = Ⓓhead /\ s R_A1 = Ⓓkey /\
-    node_distance head NULL len /\
+    s R_A0 = Ⓓhead /\ s R_A1 = Ⓓkey /\ 32 <= sp /\
+    node_distance base_mem head NULL len /\
+    LLBounds base_mem head 0 (sp ⊖ 32) /\
     cycle_count_of_trace t' = 0)
 | 0x10278 => Some (exists ctr mem curr, s V_MEM32 = Ⓜmem /\ mem Ⓓ[sp ⊖ 20] = curr /\
-    s R_S0 = Ⓓsp /\
-    node_distance head curr ctr /\
-    node_distance head NULL len /\
+    s R_S0 = Ⓓsp /\ mem Ⓓ[ msub 32 sp 24 ] = key/\ 32 <= sp /\ curr <> NULL /\
+    node_distance mem head curr ctr /\
+    node_distance mem head NULL len /\
     (ctr < len)%nat /\
     (head =? NULL) = false /\
+    LLBounds base_mem head 0 (sp ⊖ 32) /\
+    LLSame base_mem mem head /\
+    (forall fuel, key_in_linked_list mem head key fuel -> (ctr <= fuel)%nat) /\
     cycle_count_of_trace t' = 
         (* startup time *)
-        2 + 2 * time_mem + 2 + 3 * time_mem + time_branch + time_mem + time_branch +
+        ttbne + tlw + ttbne + tlw + 2*tsw  + taddi + 2*tsw + taddi +
         (* loop iterations *)
         (N.of_nat ctr) *
-        (3 * time_mem + time_branch + 4 * time_mem + time_branch))
-| 0x102b8 => Some (timing_postcondition base_mem head key t)
+        (3 * tlw + ttbne + 3 * tlw + tsw + ttbne))
+| 0x102b8 => Some (
+    (exists loc, key_in_linked_list base_mem head key loc /\ time_of_find_in_linked_list base_mem head key len (Some loc) t)
+    \/
+    (forall loc, ~key_in_linked_list base_mem head key loc /\ time_of_find_in_linked_list base_mem head key len None t))
 | _ => None end | _ => None end.
 
 Definition lifted_find_in_linked_list : program :=
@@ -163,8 +1159,11 @@ Theorem find_in_linked_list_timing:
          (SP: s R_SP = Ⓓsp)
          (A0: s R_A0 = Ⓓhead)
          (A1: s R_A1 = Ⓓkey)
+         (* Bound list length to prevent difficult wrap around cases *)
+         (SPLo: 32 <= sp)
+         (LLB: LLBounds base_mem head 0 (sp ⊖ 32))
          (* list length is finite *)
-         (LEN: node_distance head NULL len),
+         (LEN: node_distance base_mem head NULL len),
   satisfies_all 
     lifted_find_in_linked_list
     (find_in_linked_list_timing_invs s base_mem sp head key len)
@@ -174,6 +1173,18 @@ Proof using.
     intros.
     apply prove_invs.
     Local Ltac step := time rv_step.
+    Local Ltac llsame_solve :=
+        repeat (psimpl 
+                || assumption 
+                || lia
+                || apply noverlap_sum
+                || solve [eapply llsame_same; eassumption]
+                || apply noverlap_llsame 
+                || solve [eapply llsame_bounds; eassumption]
+                || lazymatch goal with
+                   | [H: LLBounds _ _ ?lo ?hi |- _] => apply noverlap_llsame_trans with (min:=lo) (max:=hi)
+                   end
+                   || match goal with [H:LLSame ?ml ?mr ?a |- LLSame ?mr ?ml ?a] => rewrite llsame_symmetry; apply H end).
 
     simpl. rewrite ENTRY. unfold entry_addr. step. now repeat split.
 
@@ -186,13 +1197,20 @@ Proof using.
     destruct_inv 32 PRE.
 
     (* 0x10250 -> 0x10278 *)
-    destruct PRE as (Mem & SP & A0 & A1 & Len & Cycles).
+    destruct PRE as (Mem & SP & A0 & A1 & SPLo & Len & Bounds & Cycles).
     repeat step.
     (* 0x10278 *) {
         exists 0%nat. eexists. exists head.
+        _noverlap_prepare.
+        elimstore.
         repeat split; auto. now psimpl.
-        constructor. eauto using node_distance_len_nonzero. 
+        now psimpl.
+        now rewrite Bool.negb_true_iff, N.eqb_neq in BC0.
+        constructor. apply llsame_distance with (mem:=base_mem); try easy; try llsame_solve.
+        eauto using node_distance_len_nonzero. 
         now apply Bool.negb_true_iff.
+        llsame_solve.
+        lia.
         hammer.
     }
 
@@ -200,37 +1218,128 @@ Proof using.
     inversion BC.
 
     (* head = null, postcondition *)
-    unfold timing_postcondition. exists 0%nat. split. 
-    apply Bool.negb_false_iff, N.eqb_eq in BC. subst.
-        constructor.
+    right. intros; split.
+    apply Bool.negb_false_iff, N.eqb_eq in BC. subst. intro H; inversion H; subst; try contradiction.
     unfold time_of_find_in_linked_list, NULL.
     hammer.
 
-    (* 0x10278 *)
-    destruct PRE as (ctr & mem & curr & Mem & Curr & S0 & Dist & Len & 
-        CtrLen & HeadNonNull & Cycles).
+    (* 0x10278 (66168)*)
+    destruct PRE as (ctr & mem & curr & Mem & Curr & S0 & Key & SPLo & CurrNNull & Dist & Len &
+        CtrLen & HeadNonNull & LLB & LLS & Fuel & Cycles).
     remember 0%nat as fuel; clear Heqfuel.
+    step. step. step.
+    step.
+        { repeat step.
+        (* next iteration *)
+          exists (S ctr). _noverlap_prepare. rewrite Curr in *. remember (mem Ⓓ[ 4 + curr ]) as next.
+          (* rewrite negb_true_iff, N.eqb_neq in *. *)
+          assert (Heqnext':next = list_node_next mem curr). 
+          { subst next; unfold list_node_next. destruct curr as [|p];[contradiction|reflexivity]. }
+          assert (WF:=distance_null_imp_well_formed _ _ _ Len).
+          assert (LenNext:node_distance mem head next (S ctr)). { rewrite Heqnext'; apply node_distance_next_S_len; try easy. }
+          repeat eexists; psimpl; auto.
+              { psimpl. rewrite N.mod_small by (subst; now apply getmem_bound).
+                now rewrite Bool.negb_true_iff, N.eqb_neq in BC0. }
+              { psimpl. rewrite N.mod_small by (subst; now apply getmem_bound).
+                apply llsame_distance with (mem:=mem); try llsame_solve. }
+              { apply llsame_distance with (mem:=mem). llsame_solve. assumption. }
+              {
+                destruct (Nat.lt_trichotomy (S ctr) len) as [Lt | [Eq | Gt]];[assumption | subst len; exfalso; clear CtrLen | lia ].
+                  enough (Contra:node_distance mem head next (S ctr)).
+                  assert (Help:=node_distance_uniq' _ _ _ _ _ _ Contra Len (eq_refl (S ctr))); now rewrite Help in BC0.
+                  apply DstSn; try easy. eapply distance_imp_diff; eassumption.
+                  now inversion LenNext.
+                  now inversion LenNext.
+              }
+              llsame_solve.
+              {
+                rewrite Bool.negb_true_iff, N.eqb_neq in BC0, BC.
+                rewrite Key in *.
+                apply fuel_le_incr with (curr:=curr); try easy.
+                apply llsame_distance with (mem:=mem); try easy; llsame_solve.
+                intros fuel' KeyIn'. specialize (Fuel fuel').
+                apply llsame_key_in with (mem':=mem) in KeyIn'. now specialize (Fuel KeyIn').
+                apply llsame_symmetry; llsame_solve.
+                unfold list_node_value. rewrite getmem_noverlap; try easy.
+                (* continue here *)
+                apply noverlap_shrink with (a1:=curr) (len1:=8); try lia.
+                eapply noverlap_llbounds_shrink; try eassumption.
+                eapply distance_imp_in.
+                eapply llsame_distance; try eassumption. now apply llsame_symmetry.
+                apply noverlap_sum; lia.
+              }
+              { (* timing condition *)
+                hammer.
+              }
     destruct (key_in_linked_list_dec base_mem head key fuel) as [IN|NOT_IN].
     (* The key does exist in the linked list *) {
-        repeat step.
-        (* next iteration *)
-            exists (S ctr). repeat eexists; auto.
-            psimpl.
-                fold (list_node_next mem (mem Ⓓ[ 4294967276 + sp ])).
-                constructor.
-            fold_big_subs. intro; rewrite H in *; rewrite <- Curr in *.
-            revert BC BC0.
-                fold (list_node_next mem (mem Ⓓ[ 4294967276 + sp ])).
-                fold_big_subs. intros. rewrite Curr in *.
-                clear - Dist Len BC0 CtrLen HeadNonNull.
-            hammer. find_rewrites. rewrite Npos_P_of_succ_nat, N.mul_succ_l.
-            unfold time_mem, time_branch. lia.
-        (* curr->next = null *)
-            unfold timing_postcondition. exists len.
-            repeat split; auto. unfold time_of_find_in_linked_list.
-            hammer. find_rewrites. unfold time_mem, time_branch. psimpl.
-            replace ctr with len. admit.
-
+        (* postcondition - reached end of list without finding key ... but the IN hyp says the key is present? *)
+        {
+          exfalso. clear - IN BC BC0 LLB LLS Dist Len CurrNNull Curr HeadNonNull Key Fuel.
+          replace (mem Ⓓ[ 4294967272 + sp ]) with (mem Ⓓ[ msub 32 sp 24 ]) in BC.
+          replace (mem Ⓓ[ 4294967276 + sp ]) with (mem Ⓓ[ msub 32 sp 20 ]) in BC, BC0.
+          rewrite Curr in *; elimstore; rewrite Bool.negb_true_iff, Bool.negb_false_iff, N.eqb_neq, N.eqb_eq in *.
+          assert (Help:len = S ctr). {
+            assert (Help2:=distance_last_node _ _ _ _ CurrNNull Dist). unfold list_node_next in Help2.
+            destruct curr as [|p];[contradiction|remember (Npos p) as curr]. rewrite BC0 in Help2; specialize (Help2 (eq_refl 0)).
+            eapply node_distance_uniq; eassumption.
+          }
+          rewrite Help in *.
+          move fuel before ctr; move curr before key; move HeadNonNull before CurrNNull.
+          remember (mem Ⓓ[ 4 + curr ]) as next. 
+          apply llsame_key_in with (mem':=mem) in IN; try assumption.
+          specialize (Fuel _ IN).
+          assert (Contra:=key_loc_lt_length _ _ _ _ _ Len IN).
+          assert (H:ctr = fuel) by lia; subst fuel.
+          assert (Help2:=key_in_linked_list_value_equal _ _ _ _ _ IN Dist).
+          rewrite Help2 in Key; unfold list_node_value in Key.
+          contradiction.
+          all: unfold msub; psimpl; reflexivity.
+        }}
+    (* The key does NOT exist in the linked list, we've reached the end. *) {
+      elimstore; right; intro.
+          move curr before sp; move n before sp; move ctr before len; move s' before s; move fuel before len.
+          move SBound before Mem; move SBound0 before Mem.
+          move BC at bottom; move LLB before SPLo; move LLS before LLB; move Cycles before t; move MDL after Cycles; move ENTRY before t.
+          move CtrLen before SPLo; move CurrNNull before CtrLen; move HeadNonNull before CurrNNull.
+          move loc before ctr.
+          assert (BC0':=BC0); assert (BC':=BC); move BC0 at bottom; move BC0' before MDL; move BC' before MDL.
+          rewrite Bool.negb_true_iff, N.eqb_neq in BC; rewrite Bool.negb_false_iff, N.eqb_eq in BC0.
+          replace (mem Ⓓ[ 4294967272 + sp ]) with (mem Ⓓ[ msub 32 sp 24 ]) in BC.
+          replace (mem Ⓓ[ 4294967276 + sp ]) with (mem Ⓓ[ msub 32 sp 20 ]) in BC, BC0.
+          all: try (unfold msub; psimpl; reflexivity).
+          rewrite Curr, Key in BC; rewrite Curr in BC0.
+          split.
+          intro H; apply (llsame_key_in _ mem) in H; revert H.
+          gdep loc; eapply key_not_in_list; try eassumption.
+          destruct curr;[contradiction|]; now unfold list_node_next.
+          now unfold list_node_value.
+          now intro.
+          enough (Help: len = S ctr). subst len.
+          unfold time_of_find_in_linked_list; hammer.
+          assert (Help2: list_node_next mem curr = NULL) by (destruct curr;[contradiction| now unfold list_node_next]).
+          assert (Help:=distance_last_node _ _ _ _ CurrNNull Dist Help2).
+          (* why does `destruct Help` introduce the `len=0` goal? *)
+          eapply node_distance_uniq; try eassumption.
+        }
     }
-Qed.
 
+      (* Found key at curr node *)
+      repeat step.
+      elimstore.
+          move curr before sp; move n before sp; move ctr before len; move s' before s; move fuel before len.
+          move SBound before Mem; move SBound0 before Mem.
+          move BC at bottom; move LLB before SPLo; move LLS before LLB; move Cycles before t; move MDL after Cycles; move ENTRY before t.
+          move CtrLen before SPLo; move CurrNNull before CtrLen; move HeadNonNull before CurrNNull.
+          assert (BC':=BC); move BC' before MDL; rewrite Bool.negb_false_iff, N.eqb_eq in BC.
+          replace (mem Ⓓ[ 4294967272 + sp ]) with (mem Ⓓ[ msub 32 sp 24 ]) in BC.
+          replace (mem Ⓓ[ 4294967276 + sp ]) with (mem Ⓓ[ msub 32 sp 20 ]) in BC.
+          all: try (unfold msub; psimpl; reflexivity).
+          rewrite Curr, Key in BC.
+          rename ctr into loc.
+          left; exists loc; split.
+          apply llsame_key_in with (mem:=mem).
+          eapply key_at_node; try eassumption. destruct curr;[contradiction|symmetry; now unfold list_node_value].
+          now rewrite llsame_symmetry.
+          unfold time_of_find_in_linked_list; hammer.
+Qed.
